@prefix : <https://sikt.no/ontology/dlr#> .
@prefix rdf: <http://www.w3.org/1999/02/22-rdf-syntax-ns#> .
@prefix rdfs: <http://www.w3.org/2000/01/rdf-schema#> .
@prefix xsd: <http://www.w3.org/2001/XMLSchema#> .

:Resource a rdfs:Class ;
  rdfs:comment "The basic resource type of DLR (Used to represent 'Resource', 'Content', 'Creator', 'Contributor', 'Authority, 'Publisher', 'Owner', 'License')" .

:UnusedProperty a rdfs:Class ;
  rdfs:comment "A property that is present in the data model, but is not used" .

:BirdOnlyProperty a rdfs:Class ;
  rdfs:comment "A property that is only used in BIRD" .

:Feature a rdfs:Class ;
  rdfs:comment "An descriptive key-value pair describing a resource" .

:FeatureKey a rdfs:Class ;
  rdfs:comment "The class of property used in DLR" .

:identifier a rdf:Property ;
  rdfs:comment "The unique identifier of a resource" ;
  rdfs:domain :Resource ;
  rdfs:range xsd:string .

:feature a rdf:Property ;
  rdfs:comment "The properties of a resource" ;
  rdfs:domain :Resource ;
  rdfs:range :Feature .

:featureKey a rdfs:Property ;
  rdfs:comment "A property value in DLR/BIRD" ;
  rdfs:domain :Feature ;
  rdfs:range :FeatureKey .

:featureValue a rdfs:Property ;
  rdfs:comment "A property value in DLR/BIRD" ;
  rdfs:domain :Feature ;
  rdfs:range xsd:string .

:dlr_access a :FeatureKey ;
  rdfs:comment "A string indicating that the usage is cleared with the creator (possible values: 'open' | 'restricted')" ;
  rdfs:domain :Feature ;
  rdfs:range xsd:string .

:dlr_app a :FeatureKey ;
  rdfs:comment "A string indicating what system this resource belongs to (possible values: 'learning' | 'research')" ;
  rdfs:domain :Feature ;
  rdfs:range xsd:string .

:dlr_authority a :FeatureKey ;
  rdfs:comment "A string containing a boolean value indicating if the resource is an Authority" ;
  rdfs:domain :Feature ;
  rdfs:range xsd:string .

:dlr_authority_entity_type a :FeatureKey ;
  rdfs:comment "A string indicating what type of BARE authority this is (possible values: 'person' | 'coorporation')" ;
  rdfs:domain :Feature ;
  rdfs:range xsd:string .

:dlr_authority_id a :FeatureKey ;
  rdfs:comment "The BARE identifier of the authority" ;
  rdfs:domain :Feature ;
  rdfs:range xsd:string .

:dlr_authority_identifier a :FeatureKey ;
  rdfs:comment "The unique identifier of an authority" ;
  rdfs:domain :Feature ;
  rdfs:range xsd:string .

:dlr_authority_name a :FeatureKey ;
  rdfs:comment "The name of the authority according to BARE" ;
  rdfs:domain :Feature ;
  rdfs:range xsd:string .

:dlr_authority_time_created a :FeatureKey ;
  rdfs:comment "A timestamp string defining when the authority was created" ;
  rdfs:domain :Feature ;
  rdfs:range xsd:string .

:dlr_content a :FeatureKey ;
  rdfs:comment "A string representing the content (uri if 'link', filename if 'file')" ;
  rdfs:domain :Feature ;
  rdfs:range xsd:string .

:dlr_content_content_type a :FeatureKey ;
  rdfs:comment "A string representing the content type (possible values: 'text', 'image', 'audio', 'video', 'application')" ;
  rdfs:domain :Feature ;
  rdfs:range xsd:string .

:dlr_content_default a :FeatureKey ;
  rdfs:comment "A string containing a boolean value indicating if this content is the default content" ;
  rdfs:domain :Feature ;
  rdfs:range xsd:string .

:dlr_content_generated a :FeatureKey ;
  rdfs:comment "A string containing a boolean value indicating if the content is generated" ;
  rdfs:domain :Feature ;
  rdfs:range xsd:string .

:dlr_content_height a :FeatureKey ;
  rdfs:comment "A numeric string containing the height of the content if applicable" ;
  rdfs:domain :Feature ;
  rdfs:range xsd:string .

:dlr_content_indexable a :FeatureKey, :BirdOnlyProperty ;
  rdfs:comment "A string containing a boolean value indicating if the content is indexable" ;
  rdfs:domain :Feature ;
  rdfs:range xsd:string .

:dlr_content_indexed a :FeatureKey, :BirdOnlyProperty ;
  rdfs:comment "A string containing a boolean value indicating if the content is indexed" ;
  rdfs:domain :Feature ;
  rdfs:range xsd:string .

:dlr_content_kaltura_presentation_id a :FeatureKey ;
  rdfs:comment "A string containing the kaltura id of the contents kaltura entry" ;
  rdfs:domain :Feature ;
  rdfs:range xsd:string .

:dlr_content_locale a :FeatureKey ;
  rdfs:comment "A string containing the locale of the content" ;
  rdfs:domain :Feature ;
  rdfs:range xsd:string .

:dlr_content_master a :FeatureKey, :BirdOnlyProperty ;
  rdfs:comment "A string containing a boolean value indicating if the content is master (initial upload/link)" ;
  rdfs:domain :Feature ;
  rdfs:range xsd:string .

:dlr_content_master_part a :FeatureKey, :BirdOnlyProperty ;
  rdfs:comment "A string specifying the content is considered master (when master content is more than one content))" ;
  rdfs:domain :Feature ;
  rdfs:range xsd:string .

:dlr_content_mime_type a :FeatureKey ;
  rdfs:comment "A string specifying the mime-type of the content" ;
  rdfs:domain :Feature ;
  rdfs:range xsd:string .

:dlr_content_original a :FeatureKey ;
  rdfs:comment "A string containing a boolean value indicating if the content is added by the creator (as opposed to generated)" ;
  rdfs:domain :Feature ;
  rdfs:range xsd:string .

:dlr_content_readme a :FeatureKey, :BirdOnlyProperty ;
  rdfs:comment "A string containing a boolean value indicating if the content is a readme" ;
  rdfs:domain :Feature ;
  rdfs:range xsd:string .

:dlr_content_replaced a :FeatureKey, :BirdOnlyProperty ;
  rdfs:comment "A string containing a boolean value indicating if the content is replaced (new version exists)" ;
  rdfs:domain :Feature ;
  rdfs:range xsd:string .

:dlr_content_sharing_link a :FeatureKey, :BirdOnlyProperty ;
  rdfs:comment "A string containing a boolean value indicating if the content is a sharing link (url to content without authorization)" ;
  rdfs:domain :Feature ;
  rdfs:range xsd:string .

:dlr_content_sharing_link_expires a :FeatureKey, :BirdOnlyProperty ;
  rdfs:comment "A timestamp string defining when the sharing link expires" ;
  rdfs:domain :Feature ;
  rdfs:range xsd:string .

:dlr_content_sharing_link_profile a :FeatureKey, :BirdOnlyProperty ;
  rdfs:comment "A string defining the sharing link profile (possible values: 'dlr_content_sharing_link_profile')" ;
  rdfs:domain :Feature ;
  rdfs:range xsd:string .

:dlr_content_sharing_link_ttlSeconds a :FeatureKey, :BirdOnlyProperty ;
  rdfs:comment "A numeric string defining ttl seconds for this sharing link" ;
  rdfs:domain :Feature ;
  rdfs:range xsd:string .

:dlr_content_sharing_link_url a :FeatureKey ;
  rdfs:comment "A string of the sharing link url" ;
  rdfs:domain :Feature ;
  rdfs:range xsd:string .

:dlr_content_size a :FeatureKey ;
  rdfs:comment "A string with the content size used for human readable presentation" ;
  rdfs:domain :Feature ;
  rdfs:range xsd:string .

:dlr_content_size_bytes a :FeatureKey ;
  rdfs:comment "A string of the content size in bytes" ;
  rdfs:domain :Feature ;
  rdfs:range xsd:string .

:dlr_content_time_created a :FeatureKey ;
  rdfs:comment "A timestamp string defining when the content was created" ;
  rdfs:domain :Feature ;
  rdfs:range xsd:string .

:dlr_content_title a :FeatureKey ;
  rdfs:comment "A string of the content title" ;
  rdfs:domain :Feature ;
  rdfs:range xsd:string .

:dlr_content_type a :FeatureKey ;
  rdfs:comment "A string indicating what type of content this is (possible values: 'file' | 'link')" ;
  rdfs:domain :Feature ;
  rdfs:range xsd:string .

:dlr_content_type_link_file a :FeatureKey ;
  rdfs:comment "A string containing a boolean value indicating if the link seems like a file url" ;
  rdfs:domain :Feature ;
  rdfs:range xsd:string .

:dlr_content_type_link_header_http_x_frame_options a :FeatureKey ;
  rdfs:comment "A string containing the x frame options header value of the content link if present (possible values: 'sameorigin' | 'deny')" ;
  rdfs:domain :Feature ;
  rdfs:range xsd:string .

:dlr_content_type_link_scheme_http a :FeatureKey ;
  rdfs:comment "A string containing a boolean value indicating if the content is a http link (as opposed to https)" ;
  rdfs:domain :Feature ;
  rdfs:range xsd:string .

:dlr_content_width a :FeatureKey ;
  rdfs:comment "A numeric string containing the width of the content if applicable" ;
  rdfs:domain :Feature ;
  rdfs:range xsd:string .

:dlr_contributor_identifier a :FeatureKey ;
  rdfs:comment "The unique identifier of a contributor" ;
  rdfs:domain :Feature ;
  rdfs:range xsd:string .

:dlr_contributor_name a :FeatureKey ;
  rdfs:comment "A string containing the name of the contributor" ;
  rdfs:domain :Feature ;
  rdfs:range xsd:string .

:dlr_contributor_type a :FeatureKey ;
  rdfs:comment "A string containing the type of the contributor (ContributorTypes...)" ;
  rdfs:domain :Feature ;
  rdfs:range xsd:string .

:dlr_creator_identifier a :FeatureKey ;
  rdfs:comment "The unique identifier of a creator" ;
  rdfs:domain :Feature ;
  rdfs:range xsd:string .

:dlr_creator_name a :FeatureKey ;
  rdfs:comment "The name of the creator" ;
  rdfs:domain :Feature ;
  rdfs:range xsd:string .

:dlr_creator_order a :FeatureKey, :BirdOnlyProperty ;
  rdfs:comment "A numeric string indicating the placement when ordering creators" ;
  rdfs:domain :Feature ;
  rdfs:range xsd:string .

:dlr_creator_time_created a :FeatureKey ;
  rdfs:comment "A timestamp string defining when the creator was created" ;
  rdfs:domain :Feature ;
  rdfs:range xsd:string .

:dlr_description a :FeatureKey ;
  rdfs:comment "A textual description of the resource" ;
  rdfs:domain :Feature ;
  rdfs:range xsd:string .

dlr_identifier a :FeatureKey ;
  rdfs:comment "The unique identifier of a resource" ;
  rdfs:domain :Feature ;
  rdfs:range xsd:string .

dlr_identifier_doi a :FeatureKey ;
  rdfs:comment "The DOI assigned to the resource" ;
  rdfs:domain :Feature ;
  rdfs:range xsd:string .

dlr_identifier_handle a :FeatureKey ;
  rdfs:comment "The Handle assigned to the resource" ;
  rdfs:domain :Feature ;
  rdfs:range xsd:string .

dlr_license_identifier a :FeatureKey ;
  rdfs:comment "The unique identifier of a license" ;
  rdfs:domain :Feature ;
  rdfs:range xsd:string .

:dlr_license a :FeatureKey ;
  rdfs:comment "A string containing a boolean value indicating if the resource is a License" ;
  rdfs:domain :Feature ;
  rdfs:range xsd:string .

:dlr_license_code a :FeatureKey ;
  rdfs:comment "A string containing the code of the license" ;
  rdfs:domain :Feature ;
  rdfs:range xsd:string .

:dlr_license_description a :FeatureKey ;
  rdfs:comment "A textual description of the license" ;
  rdfs:domain :Feature ;
  rdfs:range xsd:string .

:dlr_license_description_en a :FeatureKey ;
  rdfs:comment "A textual description of the license in english" ;
  rdfs:domain :Feature ;
  rdfs:range xsd:string .

:dlr_license_description_no a :FeatureKey ;
  rdfs:comment "A textual description of the license in norwegian" ;
  rdfs:domain :Feature ;
  rdfs:range xsd:string .

:dlr_license_issuer a :FeatureKey ;
  rdfs:comment "A string representing license issuer" ;
  rdfs:domain :Feature ;
  rdfs:range xsd:string .

:dlr_license_name a :FeatureKey ;
  rdfs:comment "A string containing the name license" ;
  rdfs:domain :Feature ;
  rdfs:range xsd:string .

:dlr_license_name_en a :FeatureKey ;
  rdfs:comment "A string containing the name license in english" ;
  rdfs:domain :Feature ;
  rdfs:range xsd:string .

:dlr_license_name_no a :FeatureKey ;
  rdfs:comment "A string containing the name license in norwegian" ;
  rdfs:domain :Feature ;
  rdfs:range xsd:string .

:dlr_license_restriction_private_access_only a :FeatureKey ;
  rdfs:comment "A string containing a boolean value indicating if the license should deny public sharing" ;
  rdfs:domain :Feature ;
  rdfs:range xsd:string .

:dlr_license_url a :FeatureKey ;
  rdfs:comment "A string containing the url to the official license details" ;
  rdfs:domain :Feature ;
  rdfs:range xsd:string .

:dlr_license_url_en a :FeatureKey ;
  rdfs:comment "A string containing the url to the official license details in english" ;
  rdfs:domain :Feature ;
  rdfs:range xsd:string .

:dlr_license_url_image a :FeatureKey ;
  rdfs:comment "A string containing an url to the license icon" ;
  rdfs:domain :Feature ;
  rdfs:range xsd:string .

:dlr_license_url_no a :FeatureKey ;
  rdfs:comment "A string containing the url to the official license details in norwegian" ;
  rdfs:domain :Feature ;
  rdfs:range xsd:string .

:dlr_licensehelper_contains_other_peoples_work a :FeatureKey ;
  rdfs:comment "A string indicating if the resource contains other people than the creator's work (possible values: 'yes' | 'no')" ;
  rdfs:domain :Feature ;
  rdfs:range xsd:string .

:dlr_licensehelper_usage_cleared_with_owner a :FeatureKey ;
  rdfs:comment "A string indicating that the usage is cleared with the creator (possible values: 'yes_other' | 'no_clearance')" ;
  rdfs:domain :Feature ;
  rdfs:range xsd:string .

:dlr_licensehelper_resource_restriction a :FeatureKey ;
  rdfs:comment "A string indicating if the creator wants to restrict usage and sharing of the resource (possible values: 'yes' | 'CC BY 4.0')" ;
  rdfs:domain :Feature ;
  rdfs:range xsd:string .

:dlr_licensehelper_others_can_modify_and_build_upon a :FeatureKey ;
  rdfs:comment "A string indicating if the creator wants to allow modifications of the resource (possible values: 'yes' | 'NC')" ;
  rdfs:domain :Feature ;
  rdfs:range xsd:string .

:dlr_licensehelper_can_be_used_commercially a :FeatureKey ;
  rdfs:comment "A string indicating if the creator allows commercial usage of the resource (possible values: 'primary_yes' | 'ND' | 'share_alike')" ;
  rdfs:domain :Feature ;
  rdfs:range xsd:string ..

:dlr_observational_count a :FeatureKey, :BirdOnlyProperty ;
  rdfs:comment "A number string defining the number of observations in a data set" ;
  rdfs:domain :Feature ;
  rdfs:range xsd:string .

:dlr_owner_identifier a :FeatureKey ;
  rdfs:comment "The unique identifier of an owner" ;
  rdfs:domain :Feature ;
  rdfs:range xsd:string .

:dlr_owner_subject a :FeatureKey ;
  rdfs:comment "The subject of an owner" ;
  rdfs:domain :Feature ;
  rdfs:range xsd:string .

:dlr_owner_time_created a :FeatureKey ;
  rdfs:comment "A timestamp string defining when the owner was created" ;
  rdfs:domain :Feature ;
  rdfs:range xsd:string .

:dlr_publication_identifier a :FeatureKey ;
  rdfs:comment "The unique identifier of a publication" ;
  rdfs:domain :Feature ;
  rdfs:range xsd:string .

:dlr_publication_publisher_identifier a :FeatureKey ;
  rdfs:comment "The unique identifier of a publication publisher" ;
  rdfs:domain :Feature ;
  rdfs:range xsd:string .

:dlr_publication_time_created a :FeatureKey ;
  rdfs:comment "A timestamp string defining when the publication was created" ;
  rdfs:domain :Feature ;
  rdfs:range xsd:string .

:dlr_publication_publisher_code a :FeatureKey ;
  rdfs:comment "A string containing the code of a publication publisher" ;
  rdfs:domain :Feature ;
  rdfs:range xsd:string .

:dlr_publisher_entity_type a :FeatureKey ;
  rdfs:comment "A string containing the type of the publisher (possible values: 'organization')" ;
  rdfs:domain :Feature ;
  rdfs:range xsd:string .

:dlr_publisher_name a :FeatureKey ;
  rdfs:comment "A string containing the name of the publisher" ;
  rdfs:domain :Feature ;
  rdfs:range xsd:string .

:dlr_publication_publisher_name a :FeatureKey ;
  rdfs:comment "A string containing the name of the publication publisher" ;
  rdfs:domain :Feature ;
  rdfs:range xsd:string .

:dlr_readme a :FeatureKey, :BirdOnlyProperty ;
  rdfs:comment "A string containing a readme text for this resource" ;
  rdfs:domain :Feature ;
  rdfs:range xsd:string .

:dlr_resource a :FeatureKey ;
  rdfs:comment "A string containing a boolean value indicating if the resource is a Resource" ;
  rdfs:domain :Feature ;
  rdfs:range xsd:string .

:dlr_resource_learning a :FeatureKey ;
  rdfs:comment "A string containing a boolean value indicating if the resource is of type learning" ;
  rdfs:domain :Feature ;
  rdfs:range xsd:string .

:dlr_status_published a :FeatureKey ;
  rdfs:comment "A string containing a boolean value indicating if the resource is published" ;
  rdfs:domain :Feature ;
  rdfs:range xsd:string .

:dlr_storage_id a :FeatureKey ;
  rdfs:comment "A string containing the institution code of publishing institution" ;
  rdfs:domain :Feature ;
  rdfs:range xsd:string .

:dlr_subject_nsi_id a :FeatureKey, :BirdOnlyProperty ;
  rdfs:comment "A Norwegian Science Index (NVI) identifier numeric string" ;
  rdfs:domain :Feature ;
  rdfs:range xsd:string .

:dlr_submitter_email a :FeatureKey ;
  rdfs:comment "A string containing the subject (user id) of the registrator" ;
  rdfs:domain :Feature ;
  rdfs:range xsd:string .

:dlr_thumbnail_default a :FeatureKey ;
  rdfs:comment "A string containing a boolean value indicating if this content thumbnail should be used for the Resource" ;
  rdfs:domain :Feature ;
  rdfs:range xsd:string .

:dlr_thumbnail_url a :FeatureKey ;
  rdfs:comment "A string containing the url of an external thumbnail for this content" ;
  rdfs:domain :Feature ;
  rdfs:range xsd:string .

:dlr_time_created a :FeatureKey ;
  rdfs:comment "A timestamp string defining when the resource was created" ;
  rdfs:domain :Feature ;
  rdfs:range xsd:string .

:dlr_time_expire a :FeatureKey, :UnusedProperty ;
  rdfs:comment "A timestamp string defining when the resource should be unpublished" ;
  rdfs:domain :Feature ;
  rdfs:range xsd:string .

:dlr_time_published a :FeatureKey ;
  rdfs:comment "A timestamp string defining when the resource was published" ;
  rdfs:domain :Feature ;
  rdfs:range xsd:string .

:dlr_title a :FeatureKey ;
  rdfs:comment "The name given to the resource by its creator" ;
  rdfs:domain :Feature ;
  rdfs:range xsd:string .

:dlr_title_alternative a :FeatureKey, :BirdOnlyProperty ;
  rdfs:comment "An alternative title for the resource, potentially a translation" ;
  rdfs:domain :Feature ;
  rdfs:range xsd:string .

:dlr_type a :FeatureKey ;
  rdfs:comment "The kind of thing the resource was initialized with, either \"file\" or \"link\"" ;
  rdfs:domain :Feature ;
  rdfs:range xsd:string .


# Resource links

:ResourceLink a rdfs:Class ;
  rdfs:comment "Resource link type describing the relationship between resources" .

:type a rdf:Property ;
  rdfs:comment """A string describing the relationship between two resources (possible values: 'AUTHORITY', 'COURSE', 'COURSE_RESOURCE',
              'ISSUE', 'JOURNAL', 'MAGAZINE', 'PROJECT', 'PROJECT_WORK_PACKAGE', 'CONTRIBUTED_BY', 'FUNDED_BY', 'FUNDER', 'CREATOR',
              'PUBLISHER', 'PUBLICATION', 'CONTRIBUTOR', 'OWNER', 'READING_LIST', 'RESOURCE_LICENSE', 'RESOURCE_LICENSED_BY',
              'RESOURCE_CONTENT', 'RESOURCE_CONTENT_OWNED_BY', 'RESOURCE_CONTENT_SHARING_LINK', 'RESOURCE_CONTAINING',
              'RESOURCE_CREATED_BY', 'RESOURCE_PUBLISHED_BY', 'RESOURCE_CONTRIBUTED_BY', 'RESOURCE_OWNED_BY', 'RESOURCE_VERSION_NEXT',
              'RESOURCE_VERSION_PREVIOUS', 'RESOURCE_CONTENT_VERSION_NEXT', 'RESOURCE_CONTENT_VERSION_PREVIOUS', 'PROJECT_OWNED_BY',
              'PROJECT_WORK_PACKAGE_OWNED_BY')""" ;
  rdfs:domain :ResourceLink ;
  rdfs:range xsd:string .

:resourceA a rdf:Property ;
  rdfs:comment "A string containing a resource identifier" ;
  rdfs:domain :ResourceLink ;
  rdfs:range xsd:string .

:resourceB a rdfs:Property ;
  rdfs:comment "A string containing a resource identifier" ;
  rdfs:domain :ResourceLink ;
  rdfs:range xsd:string .

:time a rdfs:Property ;
  rdfs:comment "A timestamp string defining when the resource link was created" ;
  rdfs:domain :ResourceLink ;
  rdfs:range xsd:string .


# Resource tags

:ResourceTag a rdfs:Class ;
  rdfs:comment "Resource tag describing a tag for a resource" .

:resourceIdentifier a rdf:Property ;
  rdfs:comment "A string containing a resource identifier" ;
  rdfs:domain :ResourceTag ;
  rdfs:range xsd:string .

:tagType a rdfs:Property ;
  rdfs:comment "A string containing a the type of this tag" ;
  rdfs:domain :ResourceTag ;
  rdfs:range xsd:string .

:tagValue a rdfs:Property ;
  rdfs:comment "A string containing the tag" ;
  rdfs:domain :ResourceTag ;
  rdfs:range xsd:string .


# User roles

:UserRole a rdfs:Class ;
  rdfs:comment "User roles for authorization" .

:user a rdf:Property ;
  rdfs:comment "A string containing the subject" ;
  rdfs:domain :UserRole ;
  rdfs:range xsd:string .

:object a rdfs:Property ;
  rdfs:comment "A string containing the object" ;
  rdfs:domain :UserRole ;
  rdfs:range xsd:string .

:role a rdfs:Property ;
  rdfs:comment "A string containing the role" ;
  rdfs:domain :UserRole ;
  rdfs:range xsd:string .

:time a rdfs:Property ;
  rdfs:comment "A timestamp string defining when the User Role should expire" ;
  rdfs:domain :UserRole ;
  rdfs:range xsd:string .



















