@prefix : <https://sikt.no/ontology/dlr#> .
@prefix rdf: <http://www.w3.org/1999/02/22-rdf-syntax-ns#> .
@prefix rdfs: <http://www.w3.org/2000/01/rdf-schema#> .
@prefix xsd: <http://www.w3.org/2001/XMLSchema#> .

:Resource a rdfs:Class ;
  rdfs:comment "The basic resource type of DLR" .

:UnusedProperty a rdfs:Class ;
  rdfs:comment "A property that is present in the data model, but is not used" .

:BirdOnlyProperty a rdfs:Class ;
  rdfs:comment "A property that is only used in BIRD" .

:Feature a rdfs:Class ;
  rdfs:comment "An descriptive key-value pair describing a resource" .

:FeatureKey a rdfs:Class ;
  rdfs:comment "The class of property used in DLR" .

:identifier a rdf:Property ;
  rdfs:comment "The unique identifier of a resource" ;
  rdfs:domain :Resource ;
  rdfs:range xsd:string .

:feature a rdf:Property ;
  rdfs:comment "The properties of a resource" ;
  rdfs:domain :Resource ;
  rdfs:range :Feature .

:featureKey a rdfs:Property ;
  rdfs:comment "A property value in DLR/BIRD" ;
  rdfs:domain :Feature ;
  rdfs:range :FeatureKey .

:featureValue a rdfs:Property ;
  rdfs:comment "A property value in DLR/BIRD" ;
  rdfs:domain :Feature ;
  rdfs:range xsd:string .

:dlr_title a :FeatureKey ;
  rdfs:comment "The name given to the resource by its creator" ;
  rdfs:domain :Feature ;
  rdfs:range xsd:string .

:dlr_description a :FeatureKey ;
  rdfs:comment "A textual description of the resource" ;
  rdfs:domain :Feature ;
  rdfs:range xsd:string .

:dlr_type a :FeatureKey ;
  rdfs:comment "The kind of thing the resource is, either \"file\" or \"link\"" ;
  rdfs:domain :Feature ;
  rdfs:range xsd:string .

:dlr_title_alternative a :FeatureKey, :BirdOnlyProperty ;
  rdfs:comment "An alternative title for the resource, potentially a translation" ;
  rdfs:domain :Feature ;
  rdfs:range xsd:string .

:dlr_subject_nsi_id a :FeatureKey, :BirdOnlyProperty ;
  rdfs:comment "A Norwegian Science Index (NVI) identifier numeric string" ;
  rdfs:domain :Feature ;
  rdfs:range xsd:string .

:dlr_time_expire a :FeatureKey, :UnusedProperty ;
  rdfs:comment "A timestamp string defining when the resource should be unpublished" ;
  rdfs:domain :Feature ;
  rdfs:range xsd:string .

:dlr_time_released a :FeatureKey, :UnusedProperty ;
  rdfs:comment "WE DO NOT KNOW" ;
  rdfs:domain :Feature ;
  rdfs:range xsd:string .

:dlr_observational_count a :FeatureKey, :BirdOnlyProperty ;
  rdfs:comment "A number string defining the number of observations in a data set" ;
  rdfs:domain :Feature ;
  rdfs:range xsd:string .

:dlr_readme a :FeatureKey, :BirdOnlyProperty ;
  rdfs:comment "WE DO NOT KNOW" ;
  rdfs:domain :Feature ;
  rdfs:range xsd:string .

:dlr_licensehelper_contains_other_peoples_work a :FeatureKey ;
  rdfs:comment "A boolean string indicating if the resource contains other people than the creator's work (possible values: FIX THIS)" ;
  rdfs:domain :Feature ;
  rdfs:range xsd:string .

:dlr_licensehelper_usage_cleared_with_owner a :FeatureKey ;
  rdfs:comment "A string indicating that the usage is cleared with the creator (possible values: FIX THIS)" ;
  rdfs:domain :Feature ;
  rdfs:range xsd:string .

:dlr_licensehelper_resource_restriction a :FeatureKey ;
  rdfs:comment "A textual description of the resource" ;
  rdfs:domain :Feature ;
  rdfs:range xsd:string .

:dlr_licensehelper_others_can_modify_and_build_upon a :FeatureKey ;
  rdfs:comment "A textual description of the resource" ;
  rdfs:domain :Feature ;
  rdfs:range xsd:string .
:dlr_licensehelper_can_be_used_commerciall a :FeatureKey ;
  rdfs:comment "A textual description of the resource" ;
  rdfs:domain :Feature ;
  rdfs:range xsd:string .

:dlr_time_published a :FeatureKey ;
  rdfs:comment "A timestamp string defining when the resource was published" ;
  rdfs:domain :Feature ;
  rdfs:range xsd:string .

:dlr_status_published a :FeatureKey ;
  rdfs:comment "A string containing a boolean value indicating if the resource is published" ;
  rdfs:domain :Feature ;
  rdfs:range xsd:string .

